\begin{align}
\vec{n} = \myvec{k-3\\-4+k^2}, c  = -k^2+7k-6
\label{eq:chapters/11/10/4/1/6}
\end{align}
\begin{enumerate}
    \item 
\begin{align}
\myvec{k-3\\-4+k^2} =\alpha\myvec{0\\1}
\implies
k =3,
\\
\implies        \myvec{0 & 5}\vec{x} =6
\end{align}
upon substituting from 
\eqref{eq:chapters/11/10/4/1/6}.

\item In this case, 
\begin{align}
\myvec{k-3\\-4+k^2} =\beta\myvec{1\\0}
	\implies k =\pm2
	\\
	\implies
        \myvec{-1 & 0}\vec{x} =4, \quad  k =2\\
        \myvec{-5 & 0}\vec{x} =-24, \quad  k =-2
\end{align}
\item 
	In this case, 
\begin{align}
	-k^2+7k-6 = 0
	\implies k =1,  k=6
	\\
	\implies
        \myvec{-2 & -3}\vec{x} =0, \quad  k =1\\
       \myvec{3 & 32}\vec{x} =0, \quad  k =6
\end{align}
\end{enumerate}
