\begin{enumerate}[label=\thesubsection.\arabic*,ref=\thesubsection.\theenumi]
\item Find the shortest distance between the lines
\begin{align}
	\frac{x+1}{7}&=\frac{y+1}{-6}=\frac{z+1}{1} \text{ and}
	\\
	\frac{x-3}{1}&=\frac{y-5}{-2}=\frac{z-7}{1}
\end{align}
    \solution
		\input{chapters/12/11/2/15/lsq.tex}
    \item Find the shortest distance between the lines whose vector equations are
    \begin{align}
\begin{split}
	\vec{x} &= \myvec{1\\2\\3} + \kappa_1\myvec{1\\-3\\2}
	\\
	\vec{x} &= \myvec{4\\5\\6} + \kappa_2\myvec{2\\3\\1}
\end{split}
        \label{eq:chapters/12/11/2/16/L2/svd}
    \end{align}
    \solution
		\input{chapters/12/11/2/16/lsq/lsq.tex}
\item Find the shortest distance between the lines $l_1$ and $l_2$ whose vector equations are 
\begin{align}
	\overrightarrow{r} &= \hat{i}+\hat{j}+\kappa(2\hat{i}-\hat{j}+\hat{k}) \text{ and}
	\\
	\overrightarrow{r} &= 2\hat{i}+\hat{j}-\hat{k}+\mu(3\hat{i}-5\hat{j}+2\hat{k}).
\end{align}
    \solution
		\input{chapters/12/11/2/e11/lsq/main.tex}
		%\input{chapters/12/11/2/e11/svd/svd.tex}
\item Find the shortest distance between the lines given by 
\begin{align}
	\overrightarrow{r}&=(8+3\kappa\hat{i}-(9+16\kappa)\hat{j}+(10+7\kappa)\hat{k} \text{ and} 
	\\
	\overrightarrow{r}&=15\hat{i}+29\hat{j}+5\hat{k}+\mu(3\hat{i}+8\hat{j}-5\hat{k}).
\end{align}
\item Find the shortest distance between the lines
\begin{align}
	\overrightarrow{r}&=(\hat{i}+2\hat{j}+\hat{k})+\kappa(\hat{i}-\hat{j}+\hat{k}) \text{ and} 
	\\
	\overrightarrow{r}&=2\hat{i}-\hat{j}-\hat{k}+\mu(2\hat{i}+\hat{j}+2\hat{k})
\end{align}
\item Find the matrix $\vec{X}$ so that $\vec{X}\myvec{1&2&3\\ 4&5&6}$= $\myvec{-7&-8&-9\\ 2&4&6}$.
\item Find the shortest distance between the lines whose vector equations are 
\begin{align} 
\overrightarrow{r}=(1-t)\hat{i}+(t-2)\hat{j}+(3-2t)\hat{k} \text{ and }\\ \overrightarrow{r}=(s+1)\hat{i}+(2s-1)\hat{j}-(2s+1)\hat{k}
\end{align}
\item Find the shortest distance between the lines $\overrightarrow{r}=6\hat{i}+2\hat{j}+2\hat{k}+\lambda(\hat{i}-2\hat{j}+2\hat{k})$ and $\overrightarrow{r}=-4\hat{i}-\hat{k}+\mu(3\hat{i}-2\hat{j}-2\hat{k})$.
\end{enumerate}
