The vertices of the triangle can be expressed using the equations
\begin{align}
	\myvec{1&1\\-1&1} \vec{A} &= \vec{0}
	\\
	\myvec{1&1\\1&0} \vec{B} &= \myvec{0\\k}
	\\
	\myvec{1&0\\-1&1} \vec{C} &= \myvec{k\\0}
\end{align}
from which
\begin{align}
\vec{A} = \myvec{0\\0},
	\vec{B}=\myvec{k\\-k},
	\vec{C}=\myvec{k\\k}
\end{align}
are trivially obtained.
Thus, 
\begin{align}
ar(ABC) &=\frac{1}{2}\norm{(\vec{A}-\vec{B})\times(\vec{A}-\vec{C})}\\
	&=\frac{1}{2}\norm{\myvec{-k\\k}\times\myvec{-k\\-k}}
=k^2
\end{align}
